#Processed by Id: cwm.py,v 1.164 2004/10/28 17:41:59 timbl Exp 
        #    using base file:/cwm/
        
#  Notation3 generation by
#       notation3.py,v 1.166 2004/10/28 17:41:59 timbl Exp

#   Base was: file:/cwm/
     @prefix : <http://www.cs.rdg.ac.uk/seequel#> .
     @prefix owl: <http://www.w3.org/2002/07/owl#> .
     @prefix rdf: <http://www.w3.org/1999/02/22-rdf-syntax-ns#> .
     @prefix rdfs: <http://www.w3.org/2000/01/rdf-schema#> .
     @prefix xsd: <http://www.w3.org/2001/XMLSchema#> .
    
    :Claim     a owl:Class;
         rdfs:comment "a statement or relation, which has not been verified."@en;
         rdfs:label "claim"@en;
         rdfs:subClassOf :Relation;
         owl:disjointWith :Fact .
    
    :Criteria     a owl:Class;
         rdfs:comment "an area in which quality can be measured in e-Learning"@en;
         rdfs:subClassOf owl:Thing .
    
    :Descriptor     a owl:Class;
         rdfs:comment "quality term used to evaluate quality."@en;
         rdfs:subClassOf owl:Thing .
    
    :ExperienceDescriptor     a owl:Class;
         rdfs:comment "an experience descriptor is more specific than a general descriptor and can be more easily be measured or assessed"@en;
         rdfs:label "experience descriptor"@en;
         rdfs:subClassOf :Descriptor .
    
    :Fact     a owl:Class;
         rdfs:comment "a verified statement or relation."@en;
         rdfs:label "fact"@en;
         rdfs:subClassOf :Relation;
         owl:disjointWith :Claim .
    
    :GeneralCriteria     a owl:Class;
         rdfs:comment "a broad area of the e-Learning domain with specific quality issues relevant to it"@en;
         rdfs:label "general criteria"@en;
         rdfs:subClassOf :Criteria .
    
    :GeneralDescriptor     a owl:Class;
         rdfs:comment "a quality term which cannot be directly measured and tends to be an abstract quality measure."@en;
         rdfs:label "general descriptor"@en;
         rdfs:subClassOf :Descriptor .
    
    :LearningExperienceArea     a owl:Class;
         rdfs:comment "an area of the learning experience, according to SEEQUEL there are three such areas in the e-Learning experience; context, sources and processes."@en;
         rdfs:label "learning experience area"@en;
         rdfs:subClassOf owl:Thing .
    
    :MemberOf     a owl:ObjectProperty;
         rdfs:comment "a group in which the person is a member"@en;
         rdfs:domain <http://xmlns.com/foaf/0.1/Person>;
         rdfs:label "member of"@en;
         rdfs:range <http://xmlns.com/foaf/0.1/Group>;
         owl:inverseOf <http://xmlns.com/foaf/0.1/member> .
    
    :Quality     a owl:Class;
         rdfs:comment "type or level of quality"@en;
         rdfs:label "quality"@en;
         rdfs:subClassOf owl:Thing;
         owl:oneOf  (
        :lowQuality 
        :highQuality  ) .
    
    :Relation     a owl:Class;
         rdfs:comment "internal class used to represent relations between properties"@en;
         rdfs:label "Relation"@en;
         rdfs:subClassOf rdf:statement,
                 [
             a owl:Restriction;
             owl:cardinality "1"^^xsd:nonNegativeInteger;
             owl:onProperty :subject ],
                 [
             a owl:Restriction;
             owl:cardinality "1"^^xsd:nonNegativeInteger;
             owl:onProperty :predicate ],
                 [
             a owl:Restriction;
             owl:cardinality "1"^^xsd:nonNegativeInteger;
             owl:onProperty :object ] .
    
    :Role     a owl:Class;
         rdfs:comment "role of an individual in a specific sector."@en;
         rdfs:label "role"@en;
         rdfs:subClassOf owl:Thing .
    
    :Sector     a owl:Class;
         rdfs:comment "the sector in which an individual works."@en;
         rdfs:label "sector"@en;
         rdfs:subClassOf owl:Thing .
    
    :SpecificCriteria     a owl:Class;
         rdfs:comment "is a specific area of the e-Learning domain that relates to quality"@en;
         rdfs:label "specific criteria"@en;
         rdfs:subClassOf :Criteria .
    
    :WorldView     a owl:Class;
         rdfs:comment "world view is a representation of the values an individual has, according to Boltanski and Thevenot there are six different world view; inspiration, domestic, opinion, civic, merchant and industrial."@en;
         rdfs:label "world view"@en;
         rdfs:subClassOf owl:Thing .
    
    :accessible     a :GeneralDescriptor;
         rdfs:label "accessible"@en .
    
    :administration     a :Sector;
         rdfs:label "administration"@en .
    
    :areaOfInterest     a owl:ObjectProperty;
         rdfs:comment "areas in which a person is particularly interested."@en;
         rdfs:domain <http://xmlns.com/foaf/0.1/Person>;
         rdfs:label "area of interest"@en;
         rdfs:range :LearningExperienceArea .
    
    :boring     a :GeneralDescriptor;
         rdfs:label "boring"@en .
    
    :challenging     a :ExperienceDescriptor;
         rdfs:label "challenging"@en .
    
    :civic     a :WorldView;
         rdfs:comment "following is a list of values for this world view: The general will, the common interest, generosity, selfabnegation, sacrifice, pride, the group, collective action, collective entities (ideas, values, symbols and institutions)."@en;
         rdfs:label "civic"@en .
    
    :classroomAssistant     a :Role;
         rdfs:label "classroom assistant"@en .
    
    :collaboration     a :ExperienceDescriptor;
         rdfs:label "collaboration"@en .
    
    :concise     a :ExperienceDescriptor;
         rdfs:label "concise"@en .
    
    :contributesTo     a owl:ObjectProperty,
                owl:TransitiveProperty;
         rdfs:comment "implication that one descriptor contributes to the other"@en;
         rdfs:domain :Descriptor;
         rdfs:label "contributes to"@en;
         rdfs:range  [
             owl:unionOf  (
            :Descriptor 
            :Quality  ) ] .
    
    :corporate     a :Sector;
         rdfs:label "corporate"@en .
    
    :culture     a :GeneralCriteria;
         rdfs:label "culture"@en .
    
    :delivery     a :GeneralCriteria;
         rdfs:label "delivery"@en .
    
    :describes     a owl:ObjectProperty;
         rdfs:comment "Indicates which area of the learning experience a quality term describes"@en;
         rdfs:domain :Descriptor;
         rdfs:label "describes"@en;
         rdfs:range :LearningExperienceArea .
    
    :designGuidancePrinciples     a :GeneralCriteria;
         rdfs:label "design guidance principles"@en .
    
    :domestic     a :WorldView;
         rdfs:comment "following is a list of values for this world view: Confidence, responsibility, merit, respectability, convention, dignity, tradition, hierarchy, rank; parents, children, generation; rules and confidence, principles; harmony; the natural; the duty."@en;
         rdfs:label "domestic"@en .
    
    :easyNavigation     a :ExperienceDescriptor;
         rdfs:label "easy navigation"@en .
    
    :easyToUse     a :GeneralDescriptor;
         rdfs:label "easy to use"@en .
    
    :effective     a :ExperienceDescriptor;
         rdfs:label "effective"@en .
    
    :efficient     a :ExperienceDescriptor;
         rdfs:label "efficient"@en .
    
    :engaging     a :GeneralDescriptor;
         rdfs:label "engaging"@en .
    
    :etManager     a :Role;
         rdfs:label "E&T manager"@en .
    
    :evaluation     a :GeneralCriteria;
         rdfs:label "evaluation"@en .
    
    :fact100     a :Fact;
         :madeBy :seequel;
         :object :highQuality;
         :predicate :contributesTo;
         :subject :accessible .
    
    :fact101     a :Fact;
         :madeBy :seequel;
         :object :lowQuality;
         :predicate :contributesTo;
         :subject :boring .
    
    :fact102     a :Fact;
         :madeBy :seequel;
         :object :learningSources;
         :predicate :describes;
         :subject :boring .
    
    :fact103     a :Fact;
         :madeBy :seequel;
         :object :interesting;
         :predicate :impliesNot;
         :subject :boring .
    
    :fact104     a :Fact;
         :madeBy :seequel;
         :object :highQuality;
         :predicate :contributesTo;
         :subject :easyToUse .
    
    :fact105     a :Fact;
         :madeBy :seequel;
         :object :learningSources;
         :predicate :describes;
         :subject :easyToUse .
    
    :fact106     a :Fact;
         :madeBy :seequel;
         :object :learningContext;
         :predicate :describes;
         :subject :engaging .
    
    :fact107     a :Fact;
         :madeBy :seequel;
         :object :interesting;
         :predicate :implies;
         :subject :engaging .
    
    :fact108     a :Fact;
         :madeBy :seequel;
         :object :highQuality;
         :predicate :contributesTo;
         :subject :flexible .
    
    :fact109     a :Fact;
         :madeBy :seequel;
         :object :learningProcesses;
         :predicate :describes;
         :subject :flexible .
    
    :fact110     a :Fact;
         :madeBy :seequel;
         :object :lowQuality;
         :predicate :contributesTo;
         :subject :inaccessible .
    
    :fact111     a :Fact;
         :madeBy :seequel;
         :object :accessible;
         :predicate :impliesNot;
         :subject :inaccessible .
    
    :fact112     a :Fact;
         :madeBy :seequel;
         :object :highQuality;
         :predicate :contributesTo;
         :subject :interesting .
    
    :fact113     a :Fact;
         :madeBy :seequel;
         :object :learningSources;
         :predicate :describes;
         :subject :interesting .
    
    :fact114     a :Fact;
         :madeBy :seequel;
         :object :learningProcesses;
         :predicate :describes;
         :subject :interesting .
    
    :fact115     a :Fact;
         :madeBy :seequel;
         :object :boring;
         :predicate :impliesNot;
         :subject :interesting .
    
    :fact116     a :Fact;
         :madeBy :seequel;
         :object :highQuality;
         :predicate :contributesTo;
         :subject :organised .
    
    :fact117     a :Fact;
         :madeBy :seequel;
         :object :learningContext;
         :predicate :describes;
         :subject :organised .
    
    :fact118     a :Fact;
         :madeBy :seequel;
         :object :highQuality;
         :predicate :contributesTo;
         :subject :respected .
    
    :fact119     a :Fact;
         :madeBy :seequel;
         :object :interesting;
         :predicate :implies;
         :subject :challenging .
    
    :fact120     a :Fact;
         :madeBy :seequel;
         :object :learningProcesses;
         :predicate :describes;
         :subject :collaboration .
    
    :fact121     a :Fact;
         :madeBy :seequel;
         :object :highQuality;
         :predicate :contributesTo;
         :subject :concise .
    
    :fact122     a :Fact;
         :madeBy :seequel;
         :object :learningSources;
         :predicate :describes;
         :subject :concise .
    
    :fact123     a :Fact;
         :madeBy :seequel;
         :object :easyToUse;
         :predicate :implies;
         :subject :concise .
    
    :fact124     a :Fact;
         :madeBy :seequel;
         :object :accessible;
         :predicate :implies;
         :subject :easyNavigation .
    
    :fact125     a :Fact;
         :madeBy :seequel;
         :object :easyToUse;
         :predicate :implies;
         :subject :easyNavigation .
    
    :fact126     a :Fact;
         :madeBy :seequel;
         :object :learningContext;
         :predicate :describes;
         :subject :easyNavigation .
    
    :fact127     a :Fact;
         :madeBy :seequel;
         :object :learningProcesses;
         :predicate :describes;
         :subject :effective .
    
    :fact128     a :Fact;
         :madeBy :seequel;
         :object :highQuality;
         :predicate :implies;
         :subject :effective .
    
    :fact129     a :Fact;
         :madeBy :seequel;
         :object :learningProcesses;
         :predicate :describes;
         :subject :efficient .
    
    :fact130     a :Fact;
         :madeBy :seequel;
         :object :interesting;
         :predicate :implies;
         :subject :fun .
    
    :fact131     a :Fact;
         :madeBy :seequel;
         :object :lowQuality;
         :predicate :implies;
         :subject :incomplete .
    
    :fact132     a :Fact;
         :madeBy :seequel;
         :object :learningSources;
         :predicate :describes;
         :subject :incomplete .
    
    :fact133     a :Fact;
         :madeBy :seequel;
         :object :engaging;
         :predicate :contributesTo;
         :subject :interactive .
    
    :fact134     a :Fact;
         :madeBy :seequel;
         :object :learningSources;
         :predicate :describes;
         :subject :interactive .
    
    :fact135     a :Fact;
         :madeBy :seequel;
         :object :interesting;
         :predicate :implies;
         :subject :interactive .
    
    :fact136     a :Fact;
         :madeBy :seequel;
         :object :boring;
         :predicate :implies;
         :subject :monotonous .
    
    :fact137     a :Fact;
         :madeBy :seequel;
         :object :learningProcesses;
         :predicate :describes;
         :subject :motivating .
    
    :fact138     a :Fact;
         :madeBy :seequel;
         :object :interesting;
         :predicate :implies;
         :subject :motivating .
    
    :fact139     a :Fact;
         :madeBy :seequel;
         :object :learningContext;
         :predicate :describes;
         :subject :nonIntuitiveLayout .
    
    :fact140     a :Fact;
         :madeBy :seequel;
         :object :learningSources;
         :predicate :describes;
         :subject :offTopic .
    
    :fact141     a :Fact;
         :madeBy :seequel;
         :object :boring;
         :predicate :implies;
         :subject :offTopic .
    
    :fact142     a :Fact;
         :madeBy :seequel;
         :object :learningContext;
         :predicate :describes;
         :subject :openMinded .
    
    :fact143     a :Fact;
         :madeBy :seequel;
         :object :flexible;
         :predicate :implies;
         :subject :openMinded .
    
    :fact144     a :Fact;
         :madeBy :seequel;
         :object :learningContext;
         :predicate :describes;
         :subject :qualifiedTeachers .
    
    :fact145     a :Fact;
         :madeBy :seequel;
         :object :respected;
         :predicate :implies;
         :subject :qualifiedTeachers .
    
    :fact146     a :Fact;
         :madeBy :seequel;
         :object :learningSources;
         :predicate :describes;
         :subject :relevant .
    
    :fact147     a :Fact;
         :madeBy :seequel;
         :object :interesting;
         :predicate :implies;
         :subject :relevant .
    
    :fact148     a :Fact;
         :madeBy :seequel;
         :object :offTopic;
         :predicate :impliesNot;
         :subject :relevant .
    
    :fact149     a :Fact;
         :madeBy :seequel;
         :object :boring;
         :predicate :implies;
         :subject :routine .
    
    :fact150     a :Fact;
         :madeBy :seequel;
         :object :learningContext;
         :predicate :describes;
         :subject :studentSupport .
    
    :fact151     a :Fact;
         :madeBy :seequel;
         :object :organised;
         :predicate :implies;
         :subject :studentSupport .
    
    :fact152     a :Fact;
         :madeBy :seequel;
         :object :learningContext;
         :predicate :describes;
         :subject :tolerantOfMistakes .
    
    :fact153     a :Fact;
         :madeBy :seequel;
         :object :flexible;
         :predicate :implies;
         :subject :tolerantOfMistakes .
    
    :fact154     a :Fact;
         :madeBy :seequel;
         :object :learningSources;
         :predicate :describes;
         :subject :tooLong .
    
    :fact155     a :Fact;
         :madeBy :seequel;
         :object :boring;
         :predicate :implies;
         :subject :tooLong .
    
    :fact156     a :Fact;
         :madeBy :seequel;
         :object :boring;
         :predicate :implies;
         :subject :tooSimple .
    
    :financialRules     a :GeneralCriteria;
         rdfs:label "financial rules"@en .
    
    :flexible     a :GeneralDescriptor;
         rdfs:label "flexible"@en .
    
    :fun     a :ExperienceDescriptor;
         rdfs:label "fun"@en .
    
    :guidanceRecruitmentTNA     a :GeneralCriteria;
         rdfs:label "guidance and recruitment in the training needs analysis"@en .
    
    :hasMade     a owl:ObjectProperty;
         rdfs:comment "claim and facts a person has made."@en;
         rdfs:domain  [
             owl:unionOf  (
            <http://xmlns.com/foaf/0.1/Group> 
            <http://xmlns.com/foaf/0.1/Person>  ) ];
         rdfs:label "has made"@en;
         rdfs:range :Relation;
         owl:inverseOf :madeBy .
    
    :hasRole     a owl:ObjectProperty;
         rdfs:comment "the role a person has in a specific sector."@en;
         rdfs:domain <http://xmlns.com/foaf/0.1/Person>;
         rdfs:label "has role"@en;
         rdfs:range :Role .
    
    :hasWorldView     a owl:ObjectProperty;
         rdfs:comment "the world view of a person"@en;
         rdfs:domain <http://xmlns.com/foaf/0.1/Person>;
         rdfs:label "has world view"@en;
         rdfs:range :WorldView .
    
    :highQuality     a :Quality;
         rdfs:label "high quality"@en;
         owl:differentFrom :lowQuality .
    
    :higherEducation     a :Sector;
         rdfs:label "higher education"@en .
    
    :ict     a :Sector;
         rdfs:label "ICT"@en .
    
    :implies     a owl:ObjectProperty,
                owl:TransitiveProperty;
         rdfs:comment "Indicates that a descriptor implies that another descriptor may also apply to the same entity being evaluated"@en;
         rdfs:domain :Descriptor;
         rdfs:label "implies"@en;
         rdfs:range  [
             owl:unionOf  (
            :Descriptor 
            :Quality  ) ] .
    
    :impliesNot     a owl:ObjectProperty;
         rdfs:comment "Indicates that a descriptor implies that another descriptor does not apply to the same entity"@en;
         rdfs:domain  [
             owl:unionOf  (
            :Descriptor 
            :Quality  ) ];
         rdfs:label "does not imply"@en;
         rdfs:range  [
             owl:unionOf  (
            :Descriptor 
            :Quality  ) ] .
    
    :inaccessible     a :GeneralDescriptor;
         rdfs:label "inaccessible"@en .
    
    :incomplete     a :ExperienceDescriptor;
         rdfs:label "incomplete"@en .
    
    :industrial     a :WorldView;
         rdfs:comment "following is a list of values for this world view: Progress, future, functionality, efficiency, optimality, performance, productivity, professionality, reliability, farsightedness, system."@en;
         rdfs:label "industrial"@en .
    
    :informalLearning     a :Sector;
         rdfs:label "informal learning"@en .
    
    :inspiration     a :WorldView;
         rdfs:comment "following is a list of values for this world view: Singularity, difference, innovation, originality, irrationality, imaginary, spirituality, unconscious, chance."@en;
         rdfs:label "inspiration"@en .
    
    :institutionalSetting     a :GeneralCriteria;
         rdfs:label "institutional setting"@en .
    
    :interactive     a :ExperienceDescriptor;
         rdfs:label "interactive"@en .
    
    :interesting     a :GeneralDescriptor;
         rdfs:label "interesting"@en .
    
    :karsten     a <http://xmlns.com/foaf/0.1/Person>;
         rdfs:comment "Karsten Oster Lundqvist"@en;
         rdfs:label "Karsten Oster Lundqvist"@en;
         <http://xmlns.com/foaf/0.1/firstName> "Karsten";
         <http://xmlns.com/foaf/0.1/surname> "Lundqvist" .
    
    :learner     a :Role;
         rdfs:label "learner"@en .
    
    :learnersRepresentative     a :Role;
         rdfs:label "learner's representative"@en .
    
    :learningContext     a :LearningExperienceArea;
         rdfs:comment "examples of learning contexts are: Institutional setting, environments, culture, legislation, values etc."@en;
         rdfs:label "learning context"@en .
    
    :learningEnvironment     a :GeneralCriteria;
         rdfs:label "learning environment"@en .
    
    :learningMaterials     a :GeneralCriteria;
         rdfs:label "learning material"@en .
    
    :learningProcesses     a :LearningExperienceArea;
         rdfs:comment "examples of learning processes are: Planning, design, delivery, evaluation etc."@en;
         rdfs:label "learning processes"@en .
    
    :learningSources     a :LearningExperienceArea;
         rdfs:comment "examples of learning sources are: Learning materials, reference materials, components, teachers, teachers qualifications etc. "@en;
         rdfs:label "learning sources"@en .
    
    :legislation     a :GeneralCriteria;
         rdfs:label "legislation"@en .
    
    :lowQuality     a :Quality;
         rdfs:label "low quality"@en .
    
    :madeBy     a owl:ObjectProperty;
         rdfs:comment "the person or group of persons who has made a claim or stated a fact."@en;
         rdfs:domain :Relation;
         rdfs:label "made by"@en;
         rdfs:range  [
             owl:unionOf  (
            <http://xmlns.com/foaf/0.1/Group> 
            <http://xmlns.com/foaf/0.1/Person>  ) ] .
    
    :merchant     a :WorldView;
         rdfs:comment "following is a list of values for this world view: Wealth, money, luxury; business, fair deals, good deals, bargain; interest, attentions to others; contract; competition, rivalry, opportunism, freedom."@en;
         rdfs:label "merchant"@en .
    
    :monotonous     a :ExperienceDescriptor;
         rdfs:label "monotonous"@en .
    
    :motivating     a :ExperienceDescriptor;
         rdfs:label "motivating"@en .
    
    :nonIntuitiveLayout     a :ExperienceDescriptor;
         rdfs:label "non-intuitive layout"@en .
    
    :object     a owl:ObjectProperty;
         rdfs:domain :Relation;
         rdfs:subPropertyOf rdf:object .
    
    :offTopic     a :ExperienceDescriptor;
         rdfs:label "off topic"@en .
    
    :openMinded     a :ExperienceDescriptor;
         rdfs:label "open minded"@en .
    
    :opinion     a :WorldView;
         rdfs:comment "following is a list of values for this world view: Image, reputation, fame, success, honour, acknowledgement, visibility, audience, credibility, identification. "@en;
         rdfs:label "opinion"@en .
    
    :organised     a :GeneralDescriptor;
         rdfs:label "organised"@en .
    
    :partOf     a owl:ObjectProperty,
                owl:TransitiveProperty;
         rdfs:comment "Indicates that a sector is a sub sector of another"@en;
         rdfs:domain :Sector;
         rdfs:label "part of"@en;
         rdfs:range :Sector .
    
    :policymaker     a :Role;
         rdfs:label "policymaker"@en .
    
    :predicate     a owl:ObjectProperty;
         rdfs:domain :Relation;
         rdfs:subPropertyOf rdf:predicate .
    
    :primaryEducation     a :Sector;
         rdfs:label "primary education"@en .
    
    :professionalAssociation     a :Sector;
         rdfs:label "professional association"@en .
    
    :publishers     a :Sector;
         rdfs:label "publishers"@en .
    
    :qualifiedTeachers     a :ExperienceDescriptor;
         rdfs:label "qualified teachers"@en .
    
    :relevant     a :ExperienceDescriptor;
         rdfs:label "relevant"@en .
    
    :respected     a :GeneralDescriptor;
         rdfs:label "respected"@en .
    
    :routine     a :ExperienceDescriptor;
         rdfs:label "routine"@en .
    
    :schoolK12     a :Sector;
         rdfs:label "school K-12"@en .
    
    :seequel     a <http://xmlns.com/foaf/0.1/Group>;
         rdfs:comment "Seequel"@en;
         rdfs:label "SEEQUEL"@en;
         <http://xmlns.com/foaf/0.1/member> :karsten .
    
    :staffCVandQualifications     a :GeneralCriteria;
         rdfs:label "supporting and teaching staff CV and qualifications"@en .
    
    :studentSupport     a :ExperienceDescriptor;
         rdfs:label "student support"@en .
    
    :subject     a owl:ObjectProperty;
         rdfs:domain :Relation;
         rdfs:subPropertyOf rdf:subject .
    
    :teacher     a :Role;
         rdfs:label "teacher"@en .
    
    :technicalLearningEnvironment     a :GeneralCriteria;
         rdfs:label "technical learning environment"@en .
    
    :tolerantOfMistakes     a :ExperienceDescriptor;
         rdfs:label "tolerant of mistankes"@en .
    
    :tooLong     a :ExperienceDescriptor;
         rdfs:label "too long"@en .
    
    :tooSimple     a :ExperienceDescriptor;
         rdfs:label "too simple"@en .
    
    :trackable     a :ExperienceDescriptor;
         rdfs:label "trackable"@en .
    
    :trainingServices     a :Sector;
         rdfs:label "training services"@en .
    
    :tutor     a :Role;
         :typeOf :teacher;
         rdfs:label "tutor"@en .
    
    :typeOf     a owl:ObjectProperty;
         rdfs:comment "Indicates that a role is a type of another role (eg tutor is a type of teacher)"@en;
         rdfs:domain :Role;
         rdfs:label "type of"@en;
         rdfs:range :Role .
    
    :usersOfCorporateTrainingServices     a :Sector;
         rdfs:label "users of corporate training services"@en .
    
    :valueSystem     a :GeneralCriteria;
         rdfs:label "value system"@en .
    
    :vocationalTraining     a :Sector;
         rdfs:label "vocational training"@en .
    
    :workInSector     a owl:ObjectProperty;
         rdfs:comment "the sector in which a person works."@en;
         rdfs:domain <http://xmlns.com/foaf/0.1/Person>;
         rdfs:label "works in sector";
         rdfs:range :Sector .
    
    <http://www.cs.rdg.ac.uk/seequel.n3>     a owl:Ontology;
         rdfs:comment "The SEEQUEL e-Learning Ontology";
         rdfs:label "e-Learning Ontology" .
    
    <http://xmlns.com/foaf/0.1/Group>     a owl:Class;
         rdfs:comment "a group of people"@en;
         rdfs:label "group"@en;
         rdfs:subClassOf owl:Thing .
    
    <http://xmlns.com/foaf/0.1/Person>     a owl:Class;
         rdfs:comment "an individual"@en;
         rdfs:label "person"@en;
         rdfs:subClassOf owl:Thing .
    
    <http://xmlns.com/foaf/0.1/firstName>     a owl:DatatypeProperty;
         rdfs:comment "the name of a person"@en;
         rdfs:domain <http://xmlns.com/foaf/0.1/Person>;
         rdfs:label "first name"@en;
         rdfs:range xsd:string .
    
    <http://xmlns.com/foaf/0.1/member>     a owl:ObjectProperty;
         rdfs:comment "a person who is a member of a group."@en;
         rdfs:domain <http://xmlns.com/foaf/0.1/Group>;
         rdfs:label "member"@en;
         rdfs:range <http://xmlns.com/foaf/0.1/Person> .
    
    <http://xmlns.com/foaf/0.1/surname>     a owl:DatatypeProperty;
         rdfs:comment "the surname of a person"@en;
         rdfs:domain <http://xmlns.com/foaf/0.1/Person>;
         rdfs:label "surname"@en;
         rdfs:range xsd:string .
    
#ENDS
