@prefix :		<http://www.cs.rdg.ac.uk/seequel#> .
@prefix owl:	<http://www.w3.org/2002/07/owl#> .
@prefix rdfs:	<http://www.w3.org/2000/01/rdf-schema#> .
@prefix rdf:	<http://www.w3.org/1999/02/22-rdf-syntax-ns#> .
@prefix xsd:	<http://www.w3.org/2001/XMLSchema#> .
@prefix foaf:	<http://xmlns.com/foaf/0.1/> .

:Quality				a				owl:Class ;
					rdfs:subClassOf		owl:Thing ;
					owl:oneOf			( 
									:lowQuality 
									:highQuality
									) ;
					rdfs:label			"quality"@en ;
					rdfs:comment		"type or level of quality"@en .
					
:LearningExperienceArea		a				owl:Class ;
					rdfs:subClassOf		owl:Thing ;
					rdfs:label			"learning experience area"@en ;
					rdfs:comment		"an area of the learning experience, according to SEEQUEL there are three such areas in the e-Learning experience; context, sources and processes."@en .

:Role					a				owl:Class ;
					rdfs:subClassOf		owl:Thing ;
					rdfs:label			"role"@en ;
					rdfs:comment		"role of an individual in a specific sector."@en .

:Sector				a				owl:Class ;
					rdfs:subClassOf		owl:Thing ;
					rdfs:label			"sector"@en ;
					rdfs:comment		"the sector in which an individual works."@en .

:WorldView				a				owl:Class ;
					rdfs:subClassOf		owl:Thing ;
					rdfs:label			"world view"@en ;
					rdfs:comment		"world view is a representation of the values an individual has, according to Boltanski and Thevenot there are six different world view; inspiration, domestic, opinion, civic, merchant and industrial."@en .

:Descriptor				a				owl:Class ;
					rdfs:subClassOf		owl:Thing ;
					rdfs:comment		"quality term used to evaluate quality."@en .

:ExperienceDescriptor		a				owl:Class ;
					rdfs:subClassOf		:Descriptor ;
					rdfs:label			"experience descriptor"@en ;
					rdfs:comment		"an experience descriptor is more specific than a general descriptor and can be more easily be measured or assessed"@en .

:GeneralDescriptor		a				owl:Class ;
					rdfs:subClassOf		:Descriptor ;
					rdfs:label			"general descriptor"@en ;
					rdfs:comment		"a quality term which cannot be directly measured and tends to be an abstract quality measure."@en .

:Criteria				a				owl:Class ;
					rdfs:subClassOf		owl:Thing ;
					rdfs:comment		"an area in which quality can be measured in e-Learning"@en .

:SpecificCriteria			a				owl:Class ;
					rdfs:subClassOf		:Criteria ;
					rdfs:label			"specific criteria"@en ;
					rdfs:comment		"is a specific area of the e-Learning domain that relates to quality"@en .

:GeneralCriteria			a				owl:Class ;
					rdfs:subClassOf		:Criteria ;
					rdfs:label			"general criteria"@en ;
					rdfs:comment		"a broad area of the e-Learning domain with specific quality issues relevant to it"@en .


foaf:Group				a				owl:Class ;
					rdfs:subClassOf		owl:Thing ;
					rdfs:label			"group"@en ;
					rdfs:comment		"a group of people"@en .

foaf:Person 			a				owl:Class ;
					rdfs:subClassOf		owl:Thing ;
					rdfs:label			"person"@en ;
					rdfs:comment		"an individual"@en .

foaf:firstName			a				owl:DatatypeProperty ;
					rdfs:domain			foaf:Person ;
					rdfs:range			xsd:string ;
					rdfs:label			"first name"@en ;
					rdfs:comment		"the name of a person"@en .

foaf:surname			a				owl:DatatypeProperty ;
					rdfs:domain			foaf:Person ;
					rdfs:range			xsd:string ;
					rdfs:label			"surname"@en ;
					rdfs:comment		"the surname of a person"@en .

foaf:member				a				owl:ObjectProperty ;
					rdfs:domain			foaf:Group ;
					rdfs:range			foaf:Person ;
					rdfs:label			"member"@en ;
					rdfs:comment		"a person who is a member of a group."@en .

:MemberOf				a				owl:ObjectProperty ;
					rdfs:domain			foaf:Person ;
					rdfs:range			foaf:Group ;
					owl:inverseOf		foaf:member ;
					rdfs:label			"member of"@en ;
					rdfs:comment		"a group in which the person is a member"@en .



:Relation				rdfs:subClassOf		rdf:statement ,
									[
									a	owl:Restriction ;
									owl:onProperty	:subject ;
									owl:cardinality	"1"^^xsd:nonNegativeInteger
									] ,
									[
									a	owl:Restriction ;
									owl:onProperty	:predicate ;
									owl:cardinality	"1"^^xsd:nonNegativeInteger
									] ,
									[
									a	owl:Restriction ;
									owl:onProperty	:object ;
									owl:cardinality	"1"^^xsd:nonNegativeInteger
									] ;
					rdfs:label			"Relation"@en ;
					rdfs:comment		"internal class used to represent relations between properties"@en .


:Claim				rdfs:subClassOf		:Relation ;
					owl:disjointWith		:Fact ;
					rdfs:label			"claim"@en ;
					rdfs:comment		"a statement or relation, which has not been verified."@en .

:Fact					rdfs:subClassOf		:Relation ;
					owl:disjointWith		:Claim ;
					rdfs:label			"fact"@en ;
					rdfs:comment		"a verified statement or relation."@en .

:subject				a				owl:ObjectProperty ;
					rdfs:subPropertyOf	rdf:subject ;
					rdfs:domain			:Relation .

:predicate				a				owl:ObjectProperty ;
					rdfs:subPropertyOf	rdf:predicate ;
					rdfs:domain			:Relation .

:object				a				owl:ObjectProperty ;
					rdfs:subPropertyOf	rdf:object ;
					rdfs:domain			:Relation .

:madeBy				a				owl:ObjectProperty ;
					rdfs:domain			:Relation ;
					rdfs:range			[ owl:unionOf ( foaf:Group foaf:Person ) ] ;
					rdfs:label			"made by"@en ;
					rdfs:comment		"the person or group of persons who has made a claim or stated a fact."@en .

:contributesTo			a				owl:ObjectProperty ,
									owl:TransitiveProperty ;
					rdfs:domain			:Descriptor ;
					rdfs:range			[ owl:unionOf ( :Descriptor :Quality ) ] ;
					rdfs:label			"contributes to"@en ;
					rdfs:comment		"implication that one descriptor contributes to the other"@en .

:describes				a				owl:ObjectProperty ;
					rdfs:domain			:Descriptor ;
					rdfs:range			:LearningExperienceArea ;
					rdfs:label			"describes"@en ;
					rdfs:comment		"Indicates which area of the learning experience a quality term describes"@en .

:implies				a				owl:ObjectProperty ,
									owl:TransitiveProperty ;
					rdfs:domain			:Descriptor ;
					rdfs:range			[ owl:unionOf ( :Descriptor :Quality ) ] ;
					rdfs:label			"implies"@en ;
					rdfs:comment		"Indicates that a descriptor implies that another descriptor may also apply to the same entity being evaluated"@en .


:impliesNot				a				owl:ObjectProperty ;
					rdfs:domain			[ owl:unionOf ( :Descriptor :Quality ) ] ;
					rdfs:range			[ owl:unionOf ( :Descriptor :Quality ) ] ;
					rdfs:label			"does not imply"@en ;
					rdfs:comment		"Indicates that a descriptor implies that another descriptor does not apply to the same entity"@en .


:partOf				a				owl:ObjectProperty ,
									owl:TransitiveProperty ;
					rdfs:domain			:Sector ;
					rdfs:range			:Sector ;
					rdfs:label			"part of"@en ;
					rdfs:comment		"Indicates that a sector is a sub sector of another"@en .

:typeOf				a				owl:ObjectProperty ;
					rdfs:domain			:Role ;
					rdfs:range			:Role ;
					rdfs:label			"type of"@en ;
					rdfs:comment		"Indicates that a role is a type of another role (eg tutor is a type of teacher)"@en .

:workInSector			a				owl:ObjectProperty ;
					rdfs:domain			foaf:Person ;
					rdfs:range			:Sector ;
					rdfs:label			"works in sector" ;
					rdfs:comment		"the sector in which a person works."@en .

:hasRole				a				owl:ObjectProperty ;
					rdfs:domain			foaf:Person ;
					rdfs:range			:Role ;
					rdfs:label			"has role"@en ;
					rdfs:comment		"the role a person has in a specific sector."@en .

:hasWorldView			a				owl:ObjectProperty ;
					rdfs:domain			foaf:Person ;
					rdfs:range			:WorldView ;
					rdfs:label			"has world view"@en ;
					rdfs:comment		"the world view of a person"@en .

:areaOfInterest			a				owl:ObjectProperty ;
					rdfs:domain			foaf:Person ;
					rdfs:range			:LearningExperienceArea ;
					rdfs:label			"area of interest"@en ;
					rdfs:comment		"areas in which a person is particularly interested."@en .

:hasMade				a				owl:ObjectProperty ;
					rdfs:domain			[ owl:unionOf ( foaf:Group foaf:Person ) ] ;
					rdfs:range			:Relation ;
					owl:inverseOf		:madeBy ;
					rdfs:label			"has made"@en ;
					rdfs:comment		"claim and facts a person has made."@en .


:boring				a				:GeneralDescriptor ;
					rdfs:label			"boring"@en .

:accessible				a				:GeneralDescriptor ;
					rdfs:label			"accessible"@en .

:easyToUse				a				:GeneralDescriptor ;
					rdfs:label			"easy to use"@en .

:engaging				a				:GeneralDescriptor ;
					rdfs:label			"engaging"@en .

:flexible				a				:GeneralDescriptor ;
					rdfs:label			"flexible"@en .

:inaccessible			a				:GeneralDescriptor ;
					rdfs:label			"inaccessible"@en .

:interesting			a				:GeneralDescriptor ;
					rdfs:label			"interesting"@en .

:organised				a				:GeneralDescriptor ;
					rdfs:label			"organised"@en .

:respected				a				:GeneralDescriptor ;
					rdfs:label			"respected"@en .
 
:challenging			a				:ExperienceDescriptor ;
					rdfs:label			"challenging"@en .

:collaboration			a				:ExperienceDescriptor ;
					rdfs:label			"collaborative"@en .

:concise				a				:ExperienceDescriptor ;
					rdfs:label			"concise"@en .

:easyNavigation			a				:ExperienceDescriptor ;
					rdfs:label			"easy to navigate"@en .

:effective				a				:ExperienceDescriptor ;
					rdfs:label			"effective"@en .

:efficient				a				:ExperienceDescriptor ;
					rdfs:label			"efficient"@en .

:fun					a				:ExperienceDescriptor ;
					rdfs:label			"fun"@en .

:incomplete				a				:ExperienceDescriptor ;
					rdfs:label			"incomplete"@en .

:interactive			a				:ExperienceDescriptor ;
					rdfs:label			"interactive"@en .

:monotonous				a				:ExperienceDescriptor ;
					rdfs:label			"monotonous"@en .

:motivating				a				:ExperienceDescriptor ;
					rdfs:label			"motivating"@en .

:nonIntuitiveLayout		a				:ExperienceDescriptor ;
					rdfs:label			"having a non-intuitive layout"@en .

:offTopic				a				:ExperienceDescriptor ;
					rdfs:label			"off topic"@en .

:openMinded				a				:ExperienceDescriptor ;
					rdfs:label			"open minded"@en .

:qualifiedTeachers		a				:ExperienceDescriptor ;
					rdfs:label			"having qualified teachers"@en .

:relevant				a				:ExperienceDescriptor ;
					rdfs:label			"relevant"@en .

:routine				a				:ExperienceDescriptor ;
					rdfs:label			"routine"@en .

:studentSupport			a				:ExperienceDescriptor ;
					rdfs:label			"supported by students"@en .

:tolerantOfMistakes		a				:ExperienceDescriptor ;
					rdfs:label			"tolerant of mistakes"@en .

:tooLong				a				:ExperienceDescriptor ;
					rdfs:label			"too long"@en .

:tooSimple				a				:ExperienceDescriptor ;
					rdfs:label			"too simple"@en .

:trackable				a				:ExperienceDescriptor ;
					rdfs:label			"trackable"@en .

:culture				a				:GeneralCriteria ;
					rdfs:label			"culture"@en .

:delivery				a				:GeneralCriteria ;
					rdfs:label			"delivery"@en .

:designGuidancePrinciples	a				:GeneralCriteria ;
					rdfs:label			"design guidance principles"@en .

:evaluation				a				:GeneralCriteria ;
					rdfs:label			"evaluation"@en .

:financialRules			a				:GeneralCriteria ;
					rdfs:label			"financial rules"@en .

:guidanceRecruitmentTNA		a				:GeneralCriteria ;
					rdfs:label			"guidance and recruitment in the training needs analysis"@en .

:institutionalSetting		a				:GeneralCriteria ;
					rdfs:label			"institutional setting"@en .

:learningEnvironment		a				:GeneralCriteria ;
					rdfs:label			"learning environment"@en .

:learningMaterials		a				:GeneralCriteria ;
					rdfs:label			"learning material"@en .

:legislation			a				:GeneralCriteria ;
					rdfs:label			"legislation"@en .

:staffCVandQualifications	a				:GeneralCriteria ;
					rdfs:label			"supporting and teaching staff CV and qualifications"@en .

:technicalLearningEnvironment	a				:GeneralCriteria ;
					rdfs:label			"technical learning environment"@en .

:valueSystem			a				:GeneralCriteria ;
					rdfs:label			"value system"@en .

:learningSources			a				:LearningExperienceArea ;
					rdfs:label			"learning sources"@en ;
					rdfs:comment		"examples of learning sources are: Learning materials, reference materials, components, teachers, teachers qualifications etc. "@en .

:learningContext			a				:LearningExperienceArea ;
					rdfs:label			"learning context"@en ;
					rdfs:comment		"examples of learning contexts are: Institutional setting, environments, culture, legislation, values etc."@en .

:learningProcesses		a				:LearningExperienceArea ;
					rdfs:label			"learning processes"@en ;
					rdfs:comment		"examples of learning processes are: Planning, design, delivery, evaluation etc."@en .

:lowQuality				a				:Quality ;
					rdfs:label			"low quality"@en .

:highQuality			a				:Quality ;
					owl:differentFrom		:lowQuality ;
					rdfs:label			"high quality"@en .

:classroomAssistant		a				:Role ;
					rdfs:label			"classroom assistant"@en .

:etManager				a				:Role ;
					rdfs:label			"E&T manager"@en .

:learner				a				:Role ;
					rdfs:label			"learner"@en .

:learnersRepresentative		a				:Role ;
					rdfs:label			"learner's representative"@en .

:policymaker			a				:Role ;
					rdfs:label			"policymaker"@en .

:teacher				a				:Role ;
					rdfs:label			"teacher"@en .

:tutor				a				:Role ;
					:typeOf			:teacher ;
					rdfs:label			"tutor"@en .

:administration			a				:Sector ;
					rdfs:label			"administration"@en .

:corporate				a				:Sector ;
					rdfs:label			"corporate"@en .

:higherEducation			a				:Sector ;
					rdfs:label			"higher education"@en .

:ict					a				:Sector ;
					rdfs:label			"ICT"@en .

:informalLearning			a				:Sector ;
					rdfs:label			"informal learning"@en .

:primaryEducation			a				:Sector ;
					rdfs:label			"primary education"@en .

:professionalAssociation	a				:Sector ;
					rdfs:label			"professional association"@en .

:publishers				a				:Sector ;
					rdfs:label			"publishers"@en .

:schoolK12				a				:Sector ;
					rdfs:label			"school K-12"@en .

:trainingServices			a				:Sector ;
					rdfs:label			"training services"@en .

:usersOfCorporateTrainingServices	a			:Sector ;
					rdfs:label			"users of corporate training services"@en .

:vocationalTraining		a				:Sector ;
					rdfs:label			"vocational training"@en .

:civic				a				:WorldView ;
					rdfs:label			"civic"@en ;
					rdfs:comment		"following is a list of values for this world view: The general will, the common interest, generosity, selfabnegation, sacrifice, pride, the group, collective action, collective entities (ideas, values, symbols and institutions)."@en .

:domestic				a				:WorldView ;
					rdfs:label			"domestic"@en ;
					rdfs:comment		"following is a list of values for this world view: Confidence, responsibility, merit, respectability, convention, dignity, tradition, hierarchy, rank; parents, children, generation; rules and confidence, principles; harmony; the natural; the duty."@en .

:industrial				a				:WorldView ;
					rdfs:label			"industrial"@en ;
					rdfs:comment		"following is a list of values for this world view: Progress, future, functionality, efficiency, optimality, performance, productivity, professionality, reliability, farsightedness, system."@en .

:inspiration			a				:WorldView ;
					rdfs:label			"inspiration"@en ;
					rdfs:comment		"following is a list of values for this world view: Singularity, difference, innovation, originality, irrationality, imaginary, spirituality, unconscious, chance."@en .

:merchant				a				:WorldView ;
					rdfs:label			"merchant"@en ;
					rdfs:comment		"following is a list of values for this world view: Wealth, money, luxury; business, fair deals, good deals, bargain; interest, attentions to others; contract; competition, rivalry, opportunism, freedom."@en .

:opinion				a				:WorldView ;
					rdfs:label			"opinion"@en ;
					rdfs:comment		"following is a list of values for this world view: Image, reputation, fame, success, honour, acknowledgement, visibility, audience, credibility, identification. "@en .



:seequel				a				foaf:Group ;
					foaf:member			:karsten ;
					rdfs:comment		"Seequel"@en ;
					rdfs:label			"SEEQUEL"@en .

:karsten				a				foaf:Person ;
					foaf:firstName		"Karsten" ;
					foaf:surname		"Lundqvist" ;
					rdfs:comment		"Karsten Oster Lundqvist"@en ;
					rdfs:label			"Karsten Oster Lundqvist"@en .

<http://www.cs.rdg.ac.uk/seequel.n3>
					a				owl:Ontology ;
					rdfs:comment		"The SEEQUEL e-Learning Ontology" ;
					rdfs:label			"e-Learning Ontology" .